# LV2 Contexts Extension
#
# Allows for an LV2 plugin to have several independent contexts, each with its
# own run callback and associated ports.
#
# Copyright (C) 2007 David Robillard
# 
# Permission is hereby granted, free of charge, to any person obtaining a
# copy of this software and associated documentation files (the "Software"),
# to deal in the Software without restriction, including without limitation
# the rights to use, copy, modify, merge, publish, distribute, sublicense,
# and/or sell copies of the Software, and to permit persons to whom the
# Software is furnished to do so, subject to the following conditions:
# 
# The above copyright notice and this permission notice shall be included
# in all copies or substantial portions of the Software.
# 
# THE SOFTWARE IS PROVIDED "AS IS", WITHOUT WARRANTY OF ANY KIND, EXPRESS OR
# IMPLIED, INCLUDING BUT NOT LIMITED TO THE WARRANTIES OF MERCHANTABILITY,
# FITNESS FOR A PARTICULAR PURPOSE AND NONINFRINGEMENT. IN NO EVENT SHALL
# THE AUTHORS OR COPYRIGHT HOLDERS BE LIABLE FOR ANY CLAIM, DAMAGES OR
# OTHER LIABILITY, WHETHER IN AN ACTION OF CONTRACT, TORT OR OTHERWISE,
# ARISING FROM, OUT OF OR IN CONNECTION WITH THE SOFTWARE OR THE USE OR
# OTHER DEALINGS IN THE SOFTWARE.

@prefix rsz:  <http://lv2plug.in/ns/ext/resize-port#> .
@prefix lv2:  <http://lv2plug.in/ns/lv2core#> .
@prefix rdf:  <http://www.w3.org/1999/02/22-rdf-syntax-ns#> .
@prefix rdfs: <http://www.w3.org/2000/01/rdf-schema#> .
@prefix xsd:  <http://www.w3.org/2001/XMLSchema> .
@prefix doap: <http://usefulinc.com/ns/doap#> .
@prefix foaf: <http://xmlns.com/foaf/0.1/> .

<http://lv2plug.in/ns/ext/resize-port>
	a lv2:Specification ;
	a lv2:Feature ;
    doap:name "LV2 Resize Port Extension" ;
	rdfs:comment """
An extension that allows LV2 plugins to request a resize of an output port.

Any host which supports this extension must pass an LV2_Feature to
the plugin's instantiate method with URI http://lv2plug.in/ns/ext/resize-port
and a pointer to a
<pre>
struct {
	void* host_handle;
	void (*resize_port)(void* host_handle, uint32_t index);
}
</pre>
where the plugin may call resize_port with the given host_handle from any
context to demand the resize of an output port buffer.  The plugin MUST call
this function from the context of the given port.

This function MAY return NULL at any time, plugins MUST gracefully handle
this situation.
""" .

rsz:asLargeAs a rdf:Property ;
    rdfs:domain  lv2:Port ;
    rdfs:range   lv2:Symbol ;
    rdfs:label   "as large as" ;
    rdfs:comment """
Indicates that a port requires at least as much buffer space as the port
with the given symbol on the same plugin instance.  This may be used for
any ports, but is generally most useful to indicate an output port must
be at least as large as some input port (because it will copy from it).
If a port is asLargeAs several ports, it is asLargeAs the largest such port
(not the sum of those ports' sizes).

The host guarantees that whenever an ObjectPort's run method is called,
any output O that is obj:asLargeAs an input I is connected to a buffer large
enough to copy I, or NULL if the port is lv2:connectionOptional.
""" .

rsz:minimumSize a rdf:Property ;
    rdfs:domain  lv2:Port ;
    rdfs:range   lv2:Symbol ;
    rdfs:label   "minimum size" ;
    rdfs:comment """
Indicates that a port requires a buffer at least this large, in bytes.
Any host that supports the resize-port feature MUST connect any port with a
minimumSize specified to a buffer at least as large as the value given for
this property.  Any host, especially those that do NOT support dynamic port
resizing, SHOULD do so or reduced functionality may result.
""" .
